Committed transcl tool for computation of transitive closures.

tools/transcl/src/MapletRecorder.cpp
@@ -1,0 +1,30 @@
+#include<iostream>
+
+#include "MapletRecorder.hpp"
+#include "main.h"
+#include "debug.h"
+
+void MapletRecorder::initialise() {
+  algorithm.clear();
+  /* When producing output for Isabelle/UTP. */
+  if (args.encode_output) {
+    outp << algorithm.vertices() << ";";
+  }
+}
+
+void MapletRecorder::record(index_t i, index_t j) {
+  /*debug << "Maplet: (" << id1 << ", " << id2 << ")" << endl;*/
+  algorithm.record(i, j);
+  /* When producing output for Isabelle/UTP. */
+  if (args.encode_output) {
+    outp << i << ";";
+    outp << j << ";";
+  }
+}
+
+void MapletRecorder::finalise() {
+  /* When producing output for Isabelle/UTP. */
+  if (args.encode_output) {
+    outp << endl;
+  }
+}
