tools/transcl/src/NullStream.cpp
@@ -1,0 +1,5 @@
+#include "NullStream.hpp"
+
+namespace std {
+  NullStream nil;
+}
