tools/transcl/src/ScanException.hpp
@@ -1,0 +1,23 @@
+#ifndef SCANEXCEPTION_HPP
+#define SCANEXCEPTION_HPP
+#include<string>
+#include<exception>
+#include<sstream>
+
+using namespace std;
+
+class ScanException : public exception, public stringstream {
+protected:
+  const int line, pos;
+
+public:
+  ScanException(int line, int pos);
+  ScanException(string msg, int line, int pos);
+  ScanException(const ScanException&);
+  ~ScanException() = default;
+
+  virtual const char *what() const noexcept;
+
+  void displayError();
+};
+#endif
