tools/transcl/src/Symtab.hpp
@@ -1,0 +1,45 @@
+#ifndef SYMTAB_HPP
+#define SYMTAB_HPP
+#include<iostream>
+#include<string>
+#include<vector>
+
+#include"TrieNode.cpp"
+
+using namespace std;
+
+template class TrieNode<int>;
+
+class Symtab {
+public:
+  /* Indices are represented by unsigned integers. */
+  typedef unsigned int index_t;
+
+protected:
+  /* Root of the trie encoding for the symbol table. */
+  TrieNode<index_t> root;
+  /* Array used to store symbols by their index. */
+  vector<string> symbols;
+  /* Counter for generating the next index. */
+  index_t counter;
+
+public:
+  Symtab();
+  ~Symtab() = default;
+
+  /* Remove all entries from the symbol table. */
+  void clear();
+
+  /* Obtain the identifier of a symobl; create if not present. */
+  index_t operator[](const string& symbol);
+
+  /* Obtain the symbol for a given identifier. */
+  string operator[](index_t symid);
+
+  /* Return the number of symbols in the table. */
+  int size();
+
+  /* Print the content of the symbol table. */
+  void print(ostream& os);
+};
+#endif
