tools/transcl/src/argp_conf.c
@@ -1,0 +1,140 @@
+#include<cstring>
+#include"errno.h"
+#include"debug.h"
+
+#include "argp_conf.h"
+
+/* Global args_t structure. */
+struct args_t args;
+
+/* Argp Setup */
+const char *argp_program_version = "transcl 1.0";
+
+const char *argp_program_bug_address = "<frank.zeyda@york.ac.uk>";
+
+const char algorithm_option_doc[] =
+  "Select the algorithm to be used. Possible values are floyd-warshall and boost, the latter using graph algorithms of the C++ Boost Library. The default value is floyd-warshall.";
+
+const char encode_option_doc[] =
+  "Encode output for reconstruction in Isabelle/HOL. Possible values for TYPE are \"rel\" and \"set\", where the latter merely outputs the range set of the closure but not the entire relation.";
+
+const char acyclic_option_doc[] =
+  "Only determine whether the relation is acyclic. This outputs either \"true\" or \"false\".";
+
+const char output_file_option_doc[] =
+  "Output to FILE instead of the standard output.";
+
+struct argp_option options[] = {
+  {"algorithm",   'a', "NAME",  0, algorithm_option_doc },
+  {"encode",      'e', "TYPE",  OPTION_ARG_OPTIONAL, encode_option_doc },
+  {"cyclic",      'c', nullptr, 0, acyclic_option_doc },
+  {"output-file", 'o', "FILE",  0, output_file_option_doc },
+  { 0 }
+};
+
+error_t parse_opt (int key, char *arg, struct argp_state *state) {
+  struct args_t *args = (struct args_t *) state->input;
+  switch (key) {
+    case 'a':
+      try {
+        args->algorithm = Algorithms.get_by_name(arg);
+      }
+      catch (invalid_argument& e) {
+        cerr << "transcl: invalid algorithm name " << "\"" << arg << "\"";
+        cerr << endl;
+        argp_state_help(state, stdout, ARGP_HELP_SEE);
+        return EINVAL;
+      }
+      break;
+
+    case 'e':
+      args->encode_output = true;
+      if (arg != nullptr) {
+        if (strcmp(arg, "rel") == 0) {
+          args->encode_mode = relation;
+        }
+        else
+        if (strcmp(arg, "set") == 0) {
+          args->encode_mode = range_set;
+        }
+        else {
+          cerr << "transcl: invalid encoding type " << "\"" << arg << "\"";
+          cerr << endl;
+          argp_state_help(state, stdout, ARGP_HELP_SEE);
+          return EINVAL;
+        }
+      }
+      break;
+
+    case 'c':
+      args->check_cyclic = true;
+      break;
+
+    case 'o':
+      args->output_file = arg;
+      break;
+
+    case ARGP_KEY_INIT:
+      debug << "ARGP_KEY_INIT" << endl;
+      break;
+
+    case ARGP_KEY_ARG:
+      debug << "ARGP_KEY_ARG" << endl;
+      if (state->arg_num == 0) {
+        args->input_file = arg;
+      }
+      else {
+        return ARGP_ERR_UNKNOWN;
+      }
+      break;
+
+    case ARGP_KEY_NO_ARGS:
+      debug << "ARGP_KEY_NO_ARGS" << endl;
+      break;
+
+    case ARGP_KEY_END:
+      debug << "ARGP_KEY_END" << endl;
+      if (args->encode_output && args->check_cyclic) {
+        cerr << "options --encode and --cyclic are mutually exclusive";
+        cerr << endl;
+        argp_state_help(state, stdout, ARGP_HELP_SEE);
+        return EINVAL;
+      }
+      break;
+
+    case ARGP_KEY_SUCCESS:
+      debug << "ARGP_KEY_SUCCESS" << endl;
+      break;
+
+    case ARGP_KEY_ERROR:
+      debug << "ARGP_KEY_ERROR" << endl;
+      break;
+
+    case ARGP_KEY_FINI:
+      debug << "ARGP_KEY_FINI" << endl;
+      break;
+
+    default:
+      return ARGP_ERR_UNKNOWN;
+  }
+  return 0;
+}
+
+const char args_doc[] = "[INPUT_FILE]";
+
+const char help_doc[] = "\n  The transcl command calculates and outputs the \
+transitive closure of a relation, supporting various algorithms. If no \
+INPUT_FILE is specified, the relation is read from the standard input. By \
+default, the result is written to the standard output, unless the option -o \
+is specified.\n\nOptions:";
+
+struct argp argp = { options, parse_opt, args_doc, help_doc };
+
+void setDefaults(args_t& args) {
+  args.algorithm = floyd_warshall;
+  args.encode_output = false;
+  args.encode_mode = relation;
+  args.check_cyclic = false;
+  args.input_file = nullptr;
+  args.output_file = nullptr;
+}
