tools/transcl/src/main.c
@@ -1,0 +1,164 @@
+#include<iostream>
+#include<fstream>
+#include<sstream>
+#include<string>
+#include<iterator>
+#include<stdexcept>
+#include<cstdlib>
+#include<cstring>
+#include<cassert>
+#include"debug.h"
+
+#include "main.h"
+
+#include "Symtab.hpp"
+#include "Scanner.hpp"
+#include "Algorithms.hpp"
+
+#define DEBUG false
+
+using namespace std;
+
+std::ofstream* file = nullptr;
+
+void openOutputFile() {
+  if (args.output_file != nullptr) {
+    try {
+      file = new ofstream();
+      file->exceptions(ifstream::failbit | ifstream::badbit);
+      file->open(args.output_file);
+    }
+    catch (ios_base::failure) {
+      cerr << "Error writing file \"" << args.output_file << "\".";
+      debug << endl;
+      exit(EXIT_FAILURE);
+    }
+  }
+}
+
+void closeOutputFile() {
+  if (args.output_file != nullptr) {
+    try {
+      file->close();
+    }
+    catch (ios_base::failure) {
+      cerr << "Error writing file \"" << args.output_file << "\".";
+      debug << endl;
+      exit(EXIT_FAILURE);
+    }
+  }
+}
+
+error_t parse_args(int argc, char *argv[]) {
+  /* Set default options */
+  setDefaults(args);
+  /* Invoke argp parser */
+  bool debug_flag = debug_enabled;
+  disable_debug();
+  /* Could this return an error? Do we need to check? */
+  error_t result = argp_parse(&argp, argc, argv, 0, 0, &args);
+  if (debug_flag) enable_debug();
+  return result;
+}
+
+void readInput(Scanner& scanner) {
+  if (args.input_file == nullptr) {
+    debug << "Terminate with [RETURN] followed by [CTRL+D]." << endl;
+    debug << "> ";
+    /* Read relation from the standard input stream. */
+    cin >> std::noskipws;
+    std::istream_iterator<char> iter(std::cin);
+    std::istream_iterator<char> end;
+    /* Can this fail and if so, in what way? */
+    scanner.fromString(string(iter, end));
+  }
+  else {
+    try {
+      scanner.readFile(args.input_file);
+    }
+    catch (ios_base::failure) {
+      cerr << "Error reading file \"" << args.input_file << "\"." << endl;
+      exit(EXIT_FAILURE);
+    }
+  }
+}
+
+void writeOutput(Symtab& symtab, TCAlgorithm& algorithm) {
+  debug << "[Transitive Closure]" << endl;
+  try {
+    if (args.encode_output) {
+      encode_mode_t mode = args.encode_mode;
+      algorithm.encode(outp, mode);
+      if (args.output_file != NULL) {
+        algorithm.encode(debug, mode);
+      }
+    }
+    else if (args.check_cyclic) {
+      algorithm.output(symtab, debug);
+      debug << endl;
+      algorithm.cyclic(outp);
+    }
+    else {
+      algorithm.output(symtab, outp);
+      if (args.output_file != NULL) {
+        algorithm.output(symtab, debug);
+      }
+    }
+    /*debug << endl;*/
+  }
+  catch (ios_base::failure) {
+    cerr << "Error writing file \"" << args.output_file << "\".";
+    debug << endl;
+    exit(EXIT_FAILURE);
+  }
+}
+
+void parseRelation(Symtab& symtab, Scanner& scanner, TCAlgorithm& algorithm) {
+  try {
+    debug << "Scanning relation (pass 1)..." << endl;
+    scanner.scanRelation(symtab);
+    debug << "[Symbol table]" << endl;
+    symtab.print(debug);
+    algorithm.init(symtab.size());
+    debug << "Scanning relation (pass 2)..." << endl;
+    MapletRecorder mrec(algorithm);
+    scanner.scanRelation(symtab, &mrec);
+    debug << "[Initial Relation]" << endl;
+    algorithm.output(symtab, debug);
+    debug << endl;
+  }
+  catch (ScanException& e) {
+    e.displayError(); debug << endl;
+    exit(EXIT_FAILURE);
+  }
+}
+
+void execute(TCAlgorithm& algorithm) {
+  debug << "Executing " << algorithm.name() << " algorithm..." << endl;
+  algorithm.execute();
+}
+
+int main(int argc, char* argv[]) {
+  if (DEBUG) enable_debug();
+  Symtab symtab;
+  TCAlgorithm *algorithm;
+  /* Parse options */
+  error_t result = parse_args(argc, argv);
+  if (result != 0) { return EXIT_FAILURE; }
+  openOutputFile();
+  /* Read input */
+  Scanner scanner;
+  readInput(scanner);
+  /* Parse Relation */
+  algorithm = Algorithms.create(args.algorithm);
+  parseRelation(symtab, scanner, *algorithm);
+  /* Execute algorithm */
+  execute(*algorithm);
+  /* Write result */
+  writeOutput(symtab, *algorithm);
+  /* Report success and clean up */
+  cerr << "[OK]"; debug << endl;
+  closeOutputFile();
+  delete algorithm;
+  return EXIT_SUCCESS;
+}
