tools/transcl/src/main.h
@@ -1,0 +1,11 @@
+#ifndef MAIN_H
+#define MAIN_H
+#include<iostream>
+#include<fstream>
+
+#include"argp_conf.h"
+
+#define outp (file != nullptr ? (*file) : std::cout)
+
+extern std::ofstream* file;
+#endif
