fmi/Interlocking.thy
@@ -14,6 +14,11 @@ begin recall_syntax
 
 (* declare One_nat_def [simp del] *)
 
+lemma inv_subst_weakening_lemma:
+"`I \<Rightarrow> s \<dagger> I` \<Longrightarrow> `I \<and> P \<Rightarrow> s \<dagger> I`"
+apply (rel_simp)
+done
+
 subsection {* Interlocking State *}
 
 alphabet ilock_state =
@@ -72,12 +77,12 @@ subsection {* Initial State *}
 
 definition init_ilock :: "ilock_state hrel" where [urel_defs]:
 "init_ilock =
-  (cdv, tc, relays, signals, switches) := (
+  ((cdv, tc, relays, signals, switches) := (
     mk_vector\<^sub>u 11 true,
     mk_vector\<^sub>u 4 false,
     mk_vector\<^sub>u 5 false,
     mk_vector\<^sub>u 3 false,
-    mk_vector\<^sub>u 5 \<guillemotleft>STRAIGHT\<guillemotright>)"
+    vector_from_list\<^sub>u [STRAIGHT, DIVERGING, DIVERGING, STRAIGHT, DIVERGING]))"
 
 subsection {* Cyclic Behaviour *}
 
@@ -151,7 +156,8 @@ lemma ilock_type_inv_rules:
  \<lbrace>ilock_type_inv \<and> P\<rbrace>S\<lbrace>ilock_type_inv\<rbrace>\<^sub>u"
 "`ilock_type_inv \<Rightarrow> s \<dagger> ilock_type_inv` \<Longrightarrow>
  `ilock_type_inv \<and> P \<Rightarrow> s \<dagger> ilock_type_inv`"
-apply (rel_simp)+
+apply (rel_simp)
+apply (erule inv_subst_weakening_lemma)
 done
 
 text {* The tactic below is a bit quicker than @{method hoare_auto}. *}
@@ -197,9 +203,9 @@ subsubsection {* Relays Invariant *}
 
 text \<open>Ensures that at most one relay can be activated at a time.\<close>
 
-definition relays_excl_inv :: "ilock_state upred" where [upred_defs]:
-"relays_excl_inv = (
-  (#\<^sub>u(&relays) =\<^sub>u \<guillemotleft>5\<guillemotright>) \<and>
+definition relays_inv :: "ilock_state upred" where [upred_defs]:
+"relays_inv = (
+  (#\<^sub>u(&relays) =\<^sub>u 5) \<and>
   (R1 \<Rightarrow> \<not> R2 \<and> \<not> R4) \<and>
   (R2 \<Rightarrow> \<not> R1 \<and> \<not> R3 \<and> \<not> R4 \<and> \<not> R5) \<and>
   (R4 \<Rightarrow> \<not> R1 \<and> \<not> R2 \<and> \<not> R3 \<and> \<not> R5) \<and>
@@ -234,9 +240,9 @@ apply (safe; clarsimp)
 apply (safe; clarsimp)
 done
 
-lemma relays_excl_inv_cases:
-"relays_excl_inv = (&relays \<in>\<^sub>u \<guillemotleft>valid_relay_states\<guillemotright>)"
-apply (unfold relays_excl_inv_def)
+lemma relays_inv_cases:
+"relays_inv = (&relays \<in>\<^sub>u \<guillemotleft>valid_relay_states\<guillemotright>)"
+apply (unfold relays_inv_def)
 apply (rel_simp)
 apply (safe; clarsimp?)
 apply (unfold valid_relay_states_def)
@@ -244,57 +250,178 @@ apply (simp_all add: eq_vector_from_list_5)
 apply (safe; clarsimp)+
 done
 
-lemma relays_excl_inv_split:
-"`relays_excl_inv \<Rightarrow> P` = `\<^bold>\<forall> v\<in>\<guillemotleft>valid_relay_states\<guillemotright> \<bullet> P\<lbrakk>\<guillemotleft>v\<guillemotright> / &relays\<rbrakk>`"
-apply (unfold relays_excl_inv_cases)
+lemma relays_inv_split:
+"`relays_inv \<Rightarrow> P` = `\<^bold>\<forall> v\<in>\<guillemotleft>valid_relay_states\<guillemotright> \<bullet> P\<lbrakk>\<guillemotleft>v\<guillemotright> / &relays\<rbrakk>`"
+apply (unfold relays_inv_cases)
 apply (pred_simp robust)
 apply (safe; clarsimp)
 done
 
-lemma relays_excl_inv_extr:
-"`relays_excl_inv \<and> P \<Rightarrow> Q` = `relays_excl_inv \<Rightarrow> P \<Rightarrow> Q`"
+lemma relays_inv_extr:
+"`relays_inv \<and> P \<Rightarrow> Q` = `relays_inv \<Rightarrow> P \<Rightarrow> Q`"
   by (simp add: impl_alt_def utp_pred_laws.sup.assoc)
+
+lemma hoare_relays_inv_split:
+"(\<And>rs. rs \<in> valid_relay_states \<Longrightarrow> \<lbrace>ilock_type_inv\<rbrace>S\<lbrakk>\<guillemotleft>rs\<guillemotright>/$relays\<rbrakk>\<lbrace>I\<rbrace>\<^sub>u) \<Longrightarrow>
+ \<lbrace>ilock_type_inv \<and> relays_inv\<rbrace>S\<lbrace>I\<rbrace>\<^sub>u"
+apply (unfold relays_inv_cases)
+apply (rel_simp)
+done
+
+method hoare_relays_inv_tac = (
+  (rule hoare_relays_inv_split),
+  (unfold valid_relay_states_def),
+  (clarsimp; safe))
 
 text {* Do \<open>,\<close>  and \<open>;\<close> have the same precedence? Are they right-associative? *}
 
-method ilock_relays_excl_inv_tac =
+method ilock_relays_inv_tac =
   (hoare_split_inv; (
-    (unfold relays_excl_inv_extr)?,
-    (unfold relays_excl_inv_cases),
+    (unfold relays_inv_extr)?,
+    (unfold relays_inv_cases),
     (rel_simp);
     (unfold valid_relay_states_def),
     (safe; simp)))
 
 paragraph {* Invariant Preservation *}
 
-lemma init_ilock_relays_excl_inv:
-"\<lbrace>true\<rbrace>init_ilock\<lbrace>relays_excl_inv\<rbrace>\<^sub>u"
+lemma init_ilock_relays_inv:
+"\<lbrace>true\<rbrace>init_ilock\<lbrace>relays_inv\<rbrace>\<^sub>u"
   unfolding init_ilock_def by (rel_simp)
 
-lemma set_relays_relays_excl_inv:
-"\<lbrace>relays_excl_inv\<rbrace>set_relays\<lbrace>relays_excl_inv\<rbrace>\<^sub>u"
-  unfolding set_relays_def by (ilock_relays_excl_inv_tac)
+lemma set_relays_relays_inv:
+"\<lbrace>relays_inv\<rbrace>set_relays\<lbrace>relays_inv\<rbrace>\<^sub>u"
+  unfolding set_relays_def by (ilock_relays_inv_tac)
 
-lemma clear_relays_relays_excl_inv:
-"\<lbrace>relays_excl_inv\<rbrace>clear_relays\<lbrace>relays_excl_inv\<rbrace>\<^sub>u"
-  unfolding clear_relays_def by (ilock_relays_excl_inv_tac)
+lemma clear_relays_relays_inv:
+"\<lbrace>relays_inv\<rbrace>clear_relays\<lbrace>relays_inv\<rbrace>\<^sub>u"
+  unfolding clear_relays_def by (ilock_relays_inv_tac)
 
-lemma set_switches_relays_excl_inv:
-"\<lbrace>relays_excl_inv\<rbrace>set_switches\<lbrace>relays_excl_inv\<rbrace>\<^sub>u"
-  unfolding set_switches_def by (ilock_relays_excl_inv_tac)
+lemma set_switches_relays_inv:
+"\<lbrace>relays_inv\<rbrace>set_switches\<lbrace>relays_inv\<rbrace>\<^sub>u"
+  unfolding set_switches_def by (ilock_relays_inv_tac)
 
-lemma set_signals_relays_excl_inv:
-"\<lbrace>relays_excl_inv\<rbrace>set_signals\<lbrace>relays_excl_inv\<rbrace>\<^sub>u"
-  unfolding set_signals_def by (ilock_relays_excl_inv_tac)
+lemma set_signals_relays_inv:
+"\<lbrace>relays_inv\<rbrace>set_signals\<lbrace>relays_inv\<rbrace>\<^sub>u"
+  unfolding set_signals_def by (ilock_relays_inv_tac)
 
-lemma "\<lbrace>relays_excl_inv\<rbrace>ilock_cycle\<lbrace>relays_excl_inv\<rbrace>\<^sub>u"
+lemma "\<lbrace>relays_inv\<rbrace>ilock_cycle\<lbrace>relays_inv\<rbrace>\<^sub>u"
 apply (unfold ilock_cycle_def)
 apply (hoare_split)
-apply (rule set_relays_relays_excl_inv)
-apply (rule clear_relays_relays_excl_inv)
-apply (rule set_switches_relays_excl_inv)
-apply (rule set_signals_relays_excl_inv)
+apply (rule set_relays_relays_inv)
+apply (rule clear_relays_relays_inv)
+apply (rule set_switches_relays_inv)
+apply (rule set_signals_relays_inv)
 done
+
+subsection {* Switches Invariant *}
+
+(*
+definition switches_inv :: "ilock_state upred" where
+[urel_defs]: "switches_inv = (
+  (#\<^sub>u(&switches) =\<^sub>u 5) \<and>
+  (SW1 =\<^sub>u \<guillemotleft>STRAIGHT\<guillemotright>) \<and>
+  ((SW2 =\<^sub>u \<guillemotleft>STRAIGHT\<guillemotright>) \<triangleleft> R3 \<or> R5 \<triangleright> (SW2 =\<^sub>u \<guillemotleft>DIVERGING\<guillemotright>)) \<and>
+  ((SW3 =\<^sub>u \<guillemotleft>STRAIGHT\<guillemotright>) \<triangleleft> R1 \<triangleright> (SW3 =\<^sub>u \<guillemotleft>DIVERGING\<guillemotright>)) \<and>
+  (SW4 =\<^sub>u \<guillemotleft>STRAIGHT\<guillemotright>) \<and>
+  ((SW5 =\<^sub>u \<guillemotleft>STRAIGHT\<guillemotright>) \<triangleleft> R2 \<or> R3 \<triangleright> (SW5 =\<^sub>u \<guillemotleft>DIVERGING\<guillemotright>))
+)"
+*)
+
+definition switches_inv :: "ilock_state upred" where
+[urel_defs]: "switches_inv = (
+  (#\<^sub>u(&switches) =\<^sub>u 5) \<and>
+  (R1 \<Rightarrow> SW1 =\<^sub>u \<guillemotleft>STRAIGHT\<guillemotright> \<and> SW3 =\<^sub>u \<guillemotleft>STRAIGHT\<guillemotright>) \<and>
+  (R2 \<Rightarrow> SW1 =\<^sub>u \<guillemotleft>STRAIGHT\<guillemotright> \<and> SW2 =\<^sub>u \<guillemotleft>DIVERGING\<guillemotright> \<and> SW3 =\<^sub>u \<guillemotleft>DIVERGING\<guillemotright> \<and> SW5 =\<^sub>u \<guillemotleft>STRAIGHT\<guillemotright>) \<and>
+  (R3 \<Rightarrow> SW2 =\<^sub>u \<guillemotleft>STRAIGHT\<guillemotright> \<and> SW4 =\<^sub>u \<guillemotleft>STRAIGHT\<guillemotright> \<and> SW5 =\<^sub>u \<guillemotleft>STRAIGHT\<guillemotright>) \<and>
+  (R4 \<Rightarrow> SW1 =\<^sub>u \<guillemotleft>STRAIGHT\<guillemotright> \<and> SW2 =\<^sub>u \<guillemotleft>DIVERGING\<guillemotright> \<and> SW3 =\<^sub>u \<guillemotleft>DIVERGING\<guillemotright> \<and> SW5 =\<^sub>u \<guillemotleft>DIVERGING\<guillemotright>) \<and>
+  (R5 \<Rightarrow> SW2 =\<^sub>u \<guillemotleft>STRAIGHT\<guillemotright> \<and> SW4 =\<^sub>u \<guillemotleft>STRAIGHT\<guillemotright> \<and> SW5 =\<^sub>u \<guillemotleft>DIVERGING\<guillemotright>)
+)"
+
+lemma switches_inv_rules:
+"`switches_inv \<Rightarrow> s \<dagger> switches_inv` \<Longrightarrow>
+ `switches_inv \<and> P \<Rightarrow> s \<dagger> switches_inv`"
+apply (erule inv_subst_weakening_lemma)
+done
+
+lemma init_ilock_switches_inv:
+"\<lbrace>true\<rbrace>init_ilock\<lbrace>switches_inv\<rbrace>\<^sub>u"
+  unfolding init_ilock_def by (rel_simp)
+
+(***********************)
+(* REVIEWED UNTIL HERE *)
+(***********************)
+
+lemma set_switches_subst_relay_simps:
+"(switches := e ;; S)\<lbrakk>\<guillemotleft>f\<guillemotright>/$relays\<rbrakk> =
+ (switches := e\<lbrakk>\<guillemotleft>f\<guillemotright>/&relays\<rbrakk> ;; (S\<lbrakk>\<guillemotleft>f\<guillemotright>/$relays\<rbrakk>))"
+"((switches := e1 \<triangleleft> b \<triangleright>\<^sub>r switches := e2) ;; R)\<lbrakk>\<guillemotleft>f\<guillemotright>/$relays\<rbrakk> =
+ ((switches := e1\<lbrakk>\<guillemotleft>f\<guillemotright>/&relays\<rbrakk> \<triangleleft> b\<lbrakk>\<guillemotleft>f\<guillemotright>/&relays\<rbrakk> \<triangleright>\<^sub>r switches := e2\<lbrakk>\<guillemotleft>f\<guillemotright>/&relays\<rbrakk>) ;; R\<lbrakk>\<guillemotleft>f\<guillemotright>/$relays\<rbrakk>)"
+apply (rel_auto)+
+apply (blast)+
+done
+
+lemma switches_assign_lemma:
+"switches := (&switches(i \<mapsto> \<guillemotleft>v\<guillemotright>)\<^sub>u)\<lbrakk>\<guillemotleft>e\<guillemotright>/&relays\<rbrakk> =
+ switches := (&switches(i\<lbrakk>\<guillemotleft>e\<guillemotright>/&relays\<rbrakk> \<mapsto> \<guillemotleft>v\<guillemotright>)\<^sub>u)"
+apply (rel_auto)
+done
+
+lemma more_simps:
+"(s \<dagger> (1::(nat, '\<alpha>) uexpr)) = 1"
+"(s \<dagger> (2::(nat, '\<alpha>) uexpr)) = 2"
+"(s \<dagger> (3::(nat, '\<alpha>) uexpr)) = 3"
+"(s \<dagger> (4::(nat, '\<alpha>) uexpr)) = 4"
+"(s \<dagger> (5::(nat, '\<alpha>) uexpr)) = 5"
+"i \<in> {1..length l} \<Longrightarrow> \<guillemotleft>vector_from_list l\<guillemotright>(\<guillemotleft>i\<guillemotright>)\<^sub>a = \<guillemotleft>l ! (i - 1)\<guillemotright>"
+"(S \<triangleleft> \<guillemotleft>True\<guillemotright> \<triangleright>\<^sub>r T) = S"
+"(S \<triangleleft> \<guillemotleft>False \<guillemotright>\<triangleright>\<^sub>r T) = T"
+apply (rel_simp)+
+done
+
+lemma
+"\<lbrace>ilock_type_inv\<rbrace>set_switches\<lbrakk>\<guillemotleft>rs\<guillemotright>/$relays\<rbrakk>\<lbrace>I\<rbrace>\<^sub>u =
+ \<lbrace>ilock_type_inv\<rbrace>set_switches\<lbrakk>\<guillemotleft>rs\<guillemotright>/$relays\<rbrakk>\<lbrace>I\<lbrakk>\<guillemotleft>rs\<guillemotright>/&relays\<rbrakk>\<rbrace>\<^sub>u"
+apply (rel_simp robust)
+sledgehammer
+oops
+
+lemma set_switches_switches_inv:
+"\<lbrace>ilock_type_inv \<and> relays_inv\<rbrace>set_switches\<lbrace>switches_inv\<rbrace>\<^sub>u"
+apply (hoare_relays_inv_tac)
+apply (unfold set_switches_def)
+apply (simp_all only: set_switches_subst_relay_simps)
+apply (simp_all add: switches_assign_lemma more_simps usubst unrest)
+apply (unfold switches_inv_def)
+apply (hoare_split_inv)
+
+profile (rel_simp robust)+
+done
+
+(***********************)
+(* REVIEWED UNTIL HERE *)
+(***********************)
+
+subsection {* Signals Invariant *}
+
+definition signals_inv :: "ilock_state upred" where [upred_defs]:
+"signals_inv = (
+  (#\<^sub>u(&signals) =\<^sub>u 3) \<and>
+  (R3 \<Leftrightarrow> &signals[1]\<^sub>u) \<and>
+  (R5 \<Leftrightarrow> &signals[2]\<^sub>u) \<and>
+  ((R1 \<or> R2 \<or> R4) \<Leftrightarrow> &signals[3]\<^sub>u))"
+
+paragraph {* Invariant Preservation *}
+
+lemma init_ilock_signals_inv:
+"\<lbrace>true\<rbrace>init_ilock\<lbrace>signals_inv\<rbrace>\<^sub>u"
+  unfolding init_ilock_def by (rel_simp)
+
+text {* I think we have to prove the switches invariant first...! *}
+
+lemma set_relays_signals_inv:
+"\<lbrace>ilock_type_inv\<rbrace>set_switches ;; set_signals\<lbrace>signals_inv\<rbrace>\<^sub>u"
+oops
 
 subsection {* Proof Experiments *}
 
